src/smtencoding/FStar.SMTEncoding.Z3.fst
@@ -603,6 +603,15 @@ let context_profile (theory:list decl) =
 
 let mk_input (fresh : bool) (theory : list decl) : string & option string & option string =
     let ver = Options.z3_version () in
+    let theory =
+      (* Add a caption with some version info. *)
+      ( Caption <|
+          BU.format3 "Z3 invocation started by F*\n\
+                      F* version: %s -- commit hash: %s\n\
+                      Z3 version (according to F*): %s"
+                        (!Options._version) (!Options._commit) ver
+      ) :: theory
+    in
     let options = z3_options ver in
     let options = options ^ (Options.z3_smtopt() |> String.concat "\n") ^ "\n\n" in
     if Options.print_z3_statistics() then context_profile theory;
@@ -619,15 +628,6 @@ let mk_input (fresh : bool) (theory : list decl) : string & option string & opti
                 theory |>
                 BU.prefix_until (function CheckSat -> true | _ -> false) |>
                 Option.get
-            in
-            let prefix =
-              (* Add a caption with some version info. *)
-              ( Caption <|
-                  BU.format3 "Z3 invocation started by F*\n\
-                              F* version: %s -- commit hash: %s\n\
-                              Z3 version (according to F*): %s"
-                                (!Options._version) (!Options._commit) ver
-              ) :: prefix
             in
             let pp = List.map (declToSmt options) in
             let suffix = check_sat::suffix in
